specs/Spec.HMAC_DRBG.Vectors.fst
@@ -72,6 +72,7 @@ type vec = {
   a: hash_alg;
   entropy_input: hex_string;
   nonce: hex_string;
+  personalization_string: hex_string;
   entropy_input_reseed: hex_string;
   returned_bits: hex_string;
 }
@@ -81,13 +82,15 @@ let test_vectors : list vec = [
   a = SHA1;
   entropy_input = "79349bbf7cdda5799557866621c91383";
   nonce = "1146733abf8c35c8";
-  entropy_input_reseed = "c7215b5b96c48e9b338c74e3e99dfedf";  
+  personalization_string = "";
+  entropy_input_reseed = "c7215b5b96c48e9b338c74e3e99dfedf";
   returned_bits = "c6a16ab8d420706f0f34ab7fec5adca9d8ca3a133e159ca6ac43c6f8a2be22834a4c0a0affb10d7194f1c1a5cf7322ec1ae0964ed4bf122746e087fdb5b3e91b3493d5bb98faed49e85f130fc8a459b7";
   };
   {
   a = SHA2_256;
   entropy_input = "06032cd5eed33f39265f49ecb142c511da9aff2af71203bffaf34a9ca5bd9c0d";
   nonce = "0e66f71edc43e42a45ad3c6fc6cdc4df";
+  personalization_string = "";
   entropy_input_reseed = "01920a4e669ed3a85ae8a33b35a74ad7fb2a6bb4cf395ce00334a9c9a5a5d552";  
   returned_bits = "76fc79fe9b50beccc991a11b5635783a83536add03c157fb30645e611c2898bb2b1bc215000209208cd506cb28da2a51bdb03826aaf2bd2335d576d519160842e7158ad0949d1a9ec3e66ea1b1a064b005de914eac2e9d4f2d72a8616a80225422918250ff66a41bd2f864a6a38cc5b6499dc43f7f2bd09e1e0f8f5885935124";
   };
@@ -95,6 +98,7 @@ let test_vectors : list vec = [
   a = SHA2_384;
   entropy_input = "096349506f3a7653d54db7ec1d09e93413edd175b6ddbeb00e56752a520ac8ff";
   nonce = "fc7983b918acadaa71a67e1624f1b502";
+  personalization_string = "";
   entropy_input_reseed = "4260a0495fdaba58aae41df82505012d480c8e4f751fd7ebc39f9becd694b2a3";
   returned_bits = "f4c7bec0c26cf3892d214549ac6f3d82f34c6966d4295099ee56166e879a70ecae130251facda351e903d877b6c5eab5153ce87ba6c7cf8bcc61cbd14cfbe34cf1ed43678aee69cd87b60e6bcb6ff48ebd44ce9e31982d8fe20aec34fa51d625f845f61056575969bf785c2ffab4dcc754f13de63423e94bad8d5e166d96a62a602d3ee4045df162028b89cac45e6207d9097f2b3ac0ab17729251985f276f1287f5c56cc9ba1a79fbdbb291f3a945fbfdbd63cf13b82ec91f7b1085b33279e3";
   };
@@ -102,6 +106,7 @@ let test_vectors : list vec = [
   a = SHA2_512;
   entropy_input = "48c121b18733af15c27e1dd9ba66a9a81a5579cdba0f5b657ec53c2b9e90bbf6";
   nonce = "bbb7c777428068fad9970891f879b1af";
+  personalization_string = "";  
   entropy_input_reseed = "e0ffefdadb9ccf990504d568bdb4d862cbe17ccce6e22dfcab8b4804fd21421a";
   returned_bits = "05da6aac7d980da038f65f392841476d37fe70fbd3e369d1f80196e66e54b8fadb1d60e1a0f3d4dc173769d75fc3410549d7a843270a54a068b4fe767d7d9a59604510a875ad1e9731c8afd0fd50b825e2c50d062576175106a9981be37e02ec7c5cd0a69aa0ca65bddaee1b0de532e10cfa1f5bf6a026e47379736a099d6750ab121dbe3622b841baf8bdcbe875c85ba4b586b8b5b57b0fecbec08c12ff2a9453c47c6e32a52103d972c62ab9affb8e728a31fcefbbccc556c0f0a35f4b10ace2d96b906e36cbb72233201e536d3e13b045187b417d2449cad1edd192e061f12d22147b0a176ea8d9c4c35404395b6502ef333a813b6586037479e0fa3c6a23";
   };
